Finish and Inline soundness proof

code/Commitment.ec
@@ -14,31 +14,27 @@ op dr : {randomness distr | is_lossless dr} as dr_ll.
 
 
 op valid_key (key : secret_key * public_key) : bool.
-(* make a predicate *)
+op verify (pk : public_key) (m : message) (c : commitment) (d : randomness) : bool.
 
 module type Committer = {
   proc * key_gen() : secret_key * public_key
   proc commit(sk : secret_key, m : message) : commitment * randomness
 }.
 
-module type Verifier = {
-  proc verify (pk : public_key, m : message, c : commitment, d : randomness): bool
-}.
 
-
-module Correctness(C : Committer, V : Verifier) = {
+module Correctness(C : Committer) = {
   proc main(m : message) : bool = {
     var sk, pk, c, d, b;
     (sk, pk) = C.key_gen();
     (c, d)   = C.commit(sk, m);
-    b        = V.verify(pk, m, c, d);
+    b        = verify pk m c d;
     return b;
   }
 
   proc key_fixed(m : message, sk : secret_key, pk : public_key) : bool = {
     var c, d, b;
     (c, d)   = C.commit(sk, m);
-    b        = V.verify(pk, m, c, d);
+    b        = verify pk m c d;
     return b;
   }
 
@@ -51,21 +47,21 @@ module Correctness(C : Committer, V : Verifier) = {
   }
 }.
 
-lemma intermediate (C <: Committer) (V <: Verifier{C}) m' &m:
-    Pr[Correctness(C,V).main(m') @ &m : res] =
-    Pr[Correctness(C,V).intermediate(m') @ &m : res].
+lemma intermediate (C <: Committer) m' &m:
+    Pr[Correctness(C).main(m') @ &m : res] =
+    Pr[Correctness(C).intermediate(m') @ &m : res].
 proof.
   byequiv=>//. proc.
   inline *. sim.
 qed.
 
-lemma key_fixed_correct (C <: Committer) (V <: Verifier{C}) m'  &m:
+lemma key_fixed_correct (C <: Committer) m'  &m:
     phoare[C.key_gen : true ==> valid_key res] = 1%r =>
-    (phoare[Correctness(C,V).key_fixed : valid_key (sk, pk) ==> res] = 1%r)
-    => Pr[Correctness(C,V).main(m') @ &m : res] = 1%r.
+    (phoare[Correctness(C).key_fixed : valid_key (sk, pk) ==> res] = 1%r)
+    => Pr[Correctness(C).main(m') @ &m : res] = 1%r.
 proof.
   move => key_gen_valid H.
-  have -> := (intermediate C V m' &m).
+  have -> := (intermediate C m' &m).
   byphoare(: m = m' ==> )=>//.
   proc.
   call H.
@@ -102,13 +98,13 @@ module type BindingAdv = {
   proc bind(sk : secret_key, pk : public_key) : commitment * message * message * randomness * randomness
 }.
 
-module BindingGame(C : Committer, V : Verifier, B : BindingAdv) = {
+module BindingGame(C : Committer, B : BindingAdv) = {
   proc main() = {
   var sk, pk, c, m, m', r, r', v, v';
     (sk, pk) = C.key_gen();
     (c, m, m', r, r') = B.bind(sk, pk);
-    v =  V.verify(pk, m, c, r);
-    v' = V.verify(pk, m', c, r');
+    v =  verify pk m c r;
+    v' = verify pk m c r';
     return (v /\ v') /\ (m <> m');
   }
 }.
